src/polytime/basic.lean
@@ -1,5 +1,6 @@
 import data.polynomial.eval
-import encode
+import tactic.expand_exists
+import complexity_class.lemmas
 
 open tree tencodable function
 open_locale tree
@@ -14,7 +15,7 @@ inductive polytime : (tree unit → tree unit) → Prop
 | comp {f₁ f₂} : polytime f₁ → polytime f₂ → polytime (f₁ ∘ f₂)
 | prec {n f} : polytime n → polytime f →
   -- Key condition: the growth of the output of `f` should be polynomially bounded
-  (∃ P : polynomial ℕ, ∀ x (m ≤ (n x).num_nodes), (f^[m] x).num_nodes ≤ P.eval x.num_nodes) →
+  (∃ p : polynomial ℕ, ∀ x (m ≤ (n x).num_nodes), (f^[m] x).num_nodes ≤ p.eval x.num_nodes) →
   polytime (λ x, f^[(n x).num_nodes] x)
 
 namespace polytime
@@ -29,7 +30,7 @@ protected theorem const : ∀ (n : tree unit), polytime (λ _, n)
 protected theorem id : polytime (λ x, x) := prec nil left (⟨polynomial.X, λ x, by simp⟩)
 
 theorem num_nodes_poly {f : tree unit → tree unit} (hf : polytime f) :
-  ∃ P : polynomial ℕ, ∀ x, (f x).num_nodes ≤ P.eval x.num_nodes :=
+  ∃ p : polynomial ℕ, ∀ x, (f x).num_nodes ≤ p.eval x.num_nodes :=
 begin
   induction hf,
   case nil { use 0, simp, },
@@ -74,175 +75,183 @@ end polytime
 
 end tree
 
-variables {α β γ γ₀ γ₁ γ₂ γ₃ γ₄ γ₅ γ₆ γ₇ : Type}
-variables [tencodable α] [tencodable β]
+def polytime : complexity_class :=
+{ prop := tree.polytime,
+  nil := tree.polytime.nil,
+  left := tree.polytime.left,
+  right := tree.polytime.right,
+  id := tree.polytime.id,
+  pair := λ f₁ f₂, tree.polytime.pair,
+  comp := λ f₁ f₂, tree.polytime.comp,
+  ite' := λ c f g, tree.polytime.ite }
 
-def polytime1 (f : α → β) : Prop :=
-∃ (f' : tree unit → tree unit), tree.polytime f' ∧ ∀ x : α, f' (encode x) = encode (f x)
+open_locale complexity_class
+localized "notation `P` := polytime" in complexity_class
 
-/-- Polynomial time functions in many arguments -/
-def polytime [has_uncurry γ α β] (f : γ) : Prop :=
-polytime1 ↿f
+@[simp] lemma tree.polytime_iff {f : tree unit → tree unit} :
+  tree.polytime f ↔ f ∈ₑ P := @complexity_class.prop_iff_mem P f
 
-def polytime_pred [has_uncurry γ α Prop] (f : γ) : Prop :=
-polytime (λ x : α, @to_bool (↿f x) (classical.dec _))
+@[complexity] lemma tree.polytime_of_polytime {f : tree unit → tree unit} (h : f ∈ₑ P) :
+  tree.polytime f := by rwa tree.polytime_iff
 
-@[simp] lemma polytime1_iff_polytime {f : α → β} : polytime1 f ↔ polytime f := iff.rfl
+class polycodable (α : Type) extends tencodable α :=
+(poly [] : tencodable.decode α ∈ₑ P)
 
-lemma polytime1_iff_polytime_pred {f : α → Prop} :
-  polytime1 (λ x, @to_bool (f x) (classical.dec _)) ↔ polytime_pred f := iff.rfl
+attribute [complexity] polycodable.poly
 
-lemma polytime_iff_polytime_pred' {f : α → Prop} [decidable_pred f] :
-  polytime (λ x, to_bool (f x)) ↔ polytime_pred f :=
-by { convert polytime1_iff_polytime_pred, ext, congr, }
+variables {α β : Type}
 
-@[simp] lemma tree.polytime.iff_polytime {f : tree unit → tree unit} :
-  tree.polytime f ↔ polytime f :=
-⟨λ pf, ⟨f, pf, λ _, rfl⟩, λ ⟨f', pf, hf⟩, pf.of_eq hf⟩
-
-namespace polytime
-
-protected theorem id : polytime (@id α) :=
-⟨_, tree.polytime.id, λ _, rfl⟩
-
-protected theorem const (x : α) :
-polytime (λ _ : β, x) := ⟨_, tree.polytime.const (encode x), λ _, rfl⟩
-
-/-- A type is considered `polycodable` if the decoding function is
-  polynomial time. -/
-class polycodable (α : Type*) extends tencodable α :=
-(prim [] : polytime (tencodable.decode α))
-
-protected lemma some : polytime (@some α) :=
-⟨_, tree.polytime.nil.pair tree.polytime.id, λ x, by simp [encode, has_uncurry.uncurry]⟩
+lemma polycodable.decode_num_nodes_le (α : Type) [polycodable α] :
+  ∃ p : polynomial ℕ, ∀ x y, decode α x = some y → (encode y).num_nodes ≤ p.eval x.num_nodes :=
+begin
+  obtain ⟨p, hp⟩ := @tree.polytime.num_nodes_poly (λ x, encode (decode α x)) (by complexity),
+  use p, intros x y h,
+  specialize hp x,
+  simp only [h, encode, of_option, num_nodes, zero_add] at hp,
+  exact nat.le_of_succ_le hp,
+end
 
 instance : polycodable (tree unit) :=
-{ prim := polytime.some }
+⟨complexity_class.decode⟩
 
-instance : polycodable unit :=
-{ prim := polytime.const _ }
+instance [polycodable α] : polycodable (option α) :=
+⟨complexity_class.option_decode (polycodable.poly α)⟩
 
-variables [tencodable γ] [tencodable γ₀] [tencodable γ₁] [tencodable γ₂]
-  [tencodable γ₃] [tencodable γ₄] [tencodable γ₅] [tencodable γ₆]
+instance [polycodable α] [polycodable β] : polycodable (α ⊕ β) :=
+⟨complexity_class.sum_decode (polycodable.poly α) (polycodable.poly β)⟩
 
-theorem comp {f : α → β} {g : γ → α} :
-  polytime f → polytime g → polytime (λ x, f (g x))
-| ⟨f', pf', hf'⟩ ⟨g', pg', hg'⟩ :=
-⟨_, pf'.comp pg', λ x, by simp [hf', hg', has_uncurry.uncurry]⟩
+instance [polycodable α] [polycodable β] : polycodable (α × β) :=
+⟨complexity_class.prod_decode (polycodable.poly α) (polycodable.poly β)⟩
 
-theorem pair {f : α → β} {g : α → γ} : polytime f → polytime g → polytime (λ x, (f x, g x))
-| ⟨f', pf', hf'⟩ ⟨g', pg', hg'⟩ :=
-⟨_, pf'.pair pg', λ x, by simp [hf', hg', encode, has_uncurry.uncurry]⟩
+lemma polycodable.mem'_iff_mem [polycodable α] [tencodable β] {γ : Type} [has_uncurry γ α β] (f : γ) :
+  f ∈ₛ P ↔ f ∈ₑ P := complexity_class.mem'_iff_mem_decode (polycodable.poly α) 
 
-theorem fst : polytime (@prod.fst α β) := ⟨_, tree.polytime.left, λ _, rfl⟩
-theorem snd : polytime (@prod.snd α β) := ⟨_, tree.polytime.right, λ _, rfl⟩
+class polysize (α : Type*) [tencodable α] :=
+(size : α → ℕ)
+(upper [] : ∃ p : polynomial ℕ, ∀ x, size x ≤ p.eval (encode x).num_nodes)
+(lower [] : ∃ p : polynomial ℕ, ∀ x, (encode x).num_nodes ≤ p.eval (size x))
 
-protected lemma ite {P : α → Prop} [decidable_pred P] {f : α → β} {g : α → β} :
-  polytime_pred P → polytime f → polytime g → polytime (λ x, if P x then f x else g x)
-| ⟨P', pP, hP⟩ ⟨f', pf, hf⟩ ⟨g', pg, hg⟩ :=
-⟨_, tree.polytime.ite pP pf pg, λ x, by by_cases P x; simp [*, encode, has_uncurry.uncurry]⟩
+lemma polysize.decode_upper (α : Type) [polycodable α] [polysize α] :
+  ∃ p : polynomial ℕ, ∀ x y, decode α x = some y → polysize.size y ≤ p.eval x.num_nodes :=
+begin
+  obtain ⟨p, hp⟩ := polycodable.decode_num_nodes_le α,
+  obtain ⟨q, hq⟩ := polysize.upper α,
+  use q.comp p,
+  intros x y h,
+  rw [polynomial.eval_comp],
+  exact (hq _).trans (q.eval_mono $ hp _ _ h),
+end
 
-/- TODO: Autogenerate these lemmas; convert following to Lean code:
-var subscript = n => String.fromCharCode(8320 + n);
+open polysize
+variables [tencodable α] [tencodable β]
 
-var template = n =>
-`theorem comp${subscript(n)} 
-  {f : ${range(n).map(m => `γ${subscript(m)}`).join(" → ") + " → α"}} 
-  ${range(n).map(m => `{g${subscript(m)} : β → γ${subscript(m)}}`).join(" ")}
-  (hf : polytime f) ${range(n).map(m => `(hg${subscript(m)}: polytime hg${subscript(m)})`).join(" ")} :
-  polytime (λ x, f ${range(n).map(m => `(g${subscript(m)} x)`).join(" ")}) :=
-  hf.comp $ ${range(n).map(m => `hg${subscript(m)}`).join(".pair $ ")}`
- 
-var template_pred = n =>
-`theorem comp${subscript(n)} 
-  {f : ${range(n).map(m => `γ${subscript(m)}`).join(" → ") + " → Prop"}} 
-  ${range(n).map(m => `{g${subscript(m)} : α → γ${subscript(m)}}`).join(" ")}
-  (hf : polytime_pred f) ${range(n).map(m => `(hg${subscript(m)}: polytime g${subscript(m)})`).join(" ")} :
-  polytime_pred (λ x, f ${range(n).map(m => `(g${subscript(m)} x)`).join(" ")}) :=
-  hf.comp $ ${range(n).map(m => `hg${subscript(m)}`).join(".pair $ ")}`
+instance : inhabited (polysize α) :=
+⟨{ size := λ x, (encode x).num_nodes,
+  upper := ⟨polynomial.X, by simp⟩,
+  lower := ⟨polynomial.X, by simp⟩ }⟩
 
- -/
-theorem comp₂ 
-  {f : γ₀ → γ₁ → α} 
-  {g₀ : β → γ₀} {g₁ : β → γ₁}
-  (hf : polytime f) (hg₀: polytime g₀) (hg₁: polytime g₁) :
-  polytime (λ x, f (g₀ x) (g₁ x)) :=
-  hf.comp $ hg₀.pair $ hg₁
+@[simps]
+instance fintype.polysize [fintype α] : polysize α :=
+{ size := λ _, 0,
+  upper := ⟨0, λ x, zero_le'⟩,
+  lower := ⟨polynomial.C ((@finset.univ α _).sup (λ x, (encode x).num_nodes)), 
+    λ x, by { simp, exact finset.le_sup (finset.mem_univ x), }⟩ }
 
-theorem comp₃ 
-  {f : γ₀ → γ₁ → γ₂ → α} 
-  {g₀ : β → γ₀} {g₁ : β → γ₁} {g₂ : β → γ₂}
-  (hf : polytime f) (hg₀: polytime g₀) (hg₁: polytime g₁) (hg₂: polytime g₂) :
-  polytime (λ x, f (g₀ x) (g₁ x) (g₂ x)) :=
-  hf.comp $ hg₀.pair $ hg₁.pair $ hg₂
+instance [polysize α] [polysize β] : polysize (α × β) :=
+begin
+  refine_struct { size := λ x : α × β, size x.1 + size x.2 },
+  { cases upper α with p hp, cases upper β with q hq,
+    use p + q, rintro ⟨x₁, x₂⟩,
+    rw polynomial.eval_add,
+    refine add_le_add ((hp _).trans $ p.eval_mono _) ((hq _).trans $ q.eval_mono _);
+    simp [encode]; linarith only, },
+  cases lower α with p hp, cases lower β with q hq,
+  use p + q + 1, rintro ⟨x₁, x₂⟩,
+  simp only [encode, num_nodes, polynomial.eval_add, polynomial.eval_one, add_le_add_iff_right],
+  exact add_le_add ((hp _).trans $ p.eval_mono le_self_add)
+    ((hq _).trans $ q.eval_mono le_add_self),
+end
 
-theorem comp₄ 
-  {f : γ₀ → γ₁ → γ₂ → γ₃ → α} 
-  {g₀ : β → γ₀} {g₁ : β → γ₁} {g₂ : β → γ₂} {g₃ : β → γ₃}
-  (hf : polytime f) (hg₀: polytime g₀) (hg₁: polytime g₁) (hg₂: polytime g₂) (hg₃: polytime g₃) :
-  polytime (λ x, f (g₀ x) (g₁ x) (g₂ x) (g₃ x)) :=
-  hf.comp $ hg₀.pair $ hg₁.pair $ hg₂.pair $ hg₃
+@[simp] lemma polysize.prod_size [polysize α] [polysize β]
+  (x : α) (y : β) : size (x, y) = size x + size y := rfl
 
-theorem comp₅ 
-  {f : γ₀ → γ₁ → γ₂ → γ₃ → γ₄ → α} 
-  {g₀ : β → γ₀} {g₁ : β → γ₁} {g₂ : β → γ₂} {g₃ : β → γ₃} {g₄ : β → γ₄}
-  (hf : polytime f) (hg₀: polytime g₀) (hg₁: polytime g₁) (hg₂: polytime g₂) (hg₃: polytime g₃) (hg₄: polytime g₄) :
-  polytime (λ x, f (g₀ x) (g₁ x) (g₂ x) (g₃ x) (g₄ x)) :=
-  hf.comp $ hg₀.pair $ hg₁.pair $ hg₂.pair $ hg₃.pair $ hg₄
+instance : polysize ℕ := default
+instance : polysize (tree unit) := default
 
-theorem comp₆ 
-  {f : γ₀ → γ₁ → γ₂ → γ₃ → γ₄ → γ₅ → α} 
-  {g₀ : β → γ₀} {g₁ : β → γ₁} {g₂ : β → γ₂} {g₃ : β → γ₃} {g₄ : β → γ₄} {g₅ : β → γ₅}
-  (hf : polytime f) (hg₀: polytime g₀) (hg₁: polytime g₁) (hg₂: polytime g₂) (hg₃: polytime g₃) (hg₄: polytime g₄) (hg₅: polytime g₅) :
-  polytime (λ x, f (g₀ x) (g₁ x) (g₂ x) (g₃ x) (g₄ x) (g₅ x)) :=
-  hf.comp $ hg₀.pair $ hg₁.pair $ hg₂.pair $ hg₃.pair $ hg₄.pair $ hg₅
+@[simp] lemma polysize_unary_nat (n : ℕ) : size n = n :=
+by simp [polysize.size]
 
-theorem comp₇ 
-  {f : γ₀ → γ₁ → γ₂ → γ₃ → γ₄ → γ₅ → γ₆ → α} 
-  {g₀ : β → γ₀} {g₁ : β → γ₁} {g₂ : β → γ₂} {g₃ : β → γ₃} {g₄ : β → γ₄} {g₅ : β → γ₅} {g₆ : β → γ₆}
-  (hf : polytime f) (hg₀: polytime g₀) (hg₁: polytime g₁) (hg₂: polytime g₂) (hg₃: polytime g₃) (hg₄: polytime g₄) (hg₅: polytime g₅) (hg₆: polytime g₆) :
-  polytime (λ x, f (g₀ x) (g₁ x) (g₂ x) (g₃ x) (g₄ x) (g₅ x) (g₆ x)) :=
-  hf.comp $ hg₀.pair $ hg₁.pair $ hg₂.pair $ hg₃.pair $ hg₄.pair $ hg₅.pair $ hg₆
+@[simp] lemma polysize_tree_unit (x : tree unit) : size x = x.num_nodes := rfl
 
-end polytime
+def polysize_uniform [polysize α] [polysize β] (f : α → β → β) : Prop :=
+∃ (p : polynomial ℕ), ∀ x y, size (f x y) ≤ size y + p.eval (size x)
 
-namespace polytime_pred
-variables [tencodable γ] [tencodable γ₀] [tencodable γ₁] [tencodable γ₂]
-  [tencodable γ₃] [tencodable γ₄] [tencodable γ₅] [tencodable γ₆]
+theorem polysize_uniform.iterate [polysize α] [polysize β] {f : α → β → β} {n : α → ℕ}
+  (hf : polysize_uniform f) (hn : ∃ p : polynomial ℕ, ∀ x, n x ≤ p.eval (size x)) :
+    ∃ p : mv_polynomial (fin 2) ℕ, ∀ x y, size ((f x)^[n x] y) ≤ mv_polynomial.eval ![size x, size y] p :=
+begin
+  cases hn with p hn, cases hf with q hf,
+  use (mv_polynomial.X 1 + (polynomial.to_mv 0 p) * (polynomial.to_mv 0 q) : mv_polynomial (fin 2) ℕ),
+  intros x y, specialize hn x,
+  have : ∀ n : ℕ, size ((f x)^[n] y) ≤ size y + n * (q.eval $ size x),
+  { intro n, induction n with n ih, 
+    { simp, },
+    rw [iterate_succ_apply', nat.succ_mul, ← add_assoc],
+    refine (hf x _).trans _,
+    simpa using ih, },
+  refine (this $ n x).trans _,
+  simp, mono, exact zero_le',
+end
 
-theorem comp
-  {f : γ₀ → Prop} 
-  {g₀ : α → γ₀}
-  (hf : polytime_pred f) (hg₀: polytime g₀) :
-  polytime_pred (λ x, f (g₀ x)) :=
-  hf.comp $ hg₀
+lemma iterate_aux {α : Type} [polycodable α] [polysize α] (n : α → tree unit) (f : α → α) (hn : n ∈ₑ P)
+  (hf : f ∈ₑ P) (H : ∃ p : polynomial ℕ, ∀ x (m ≤ (n x).num_nodes), size (f^[m] x) ≤ p.eval (size x)) :
+  polytime.mem (λ x, f^[(n x).num_nodes] x) :=
+begin
+  -- TODO: Extract into definition (maybe?)
+  -- A version of f and n which fail "safely" (i.e. if you input something that
+  --  decodes to `none`, the output is `nil`)
+  set f' : tree unit → tree unit := λ s, (encode $ (decode α s).map f).right,
+  set n' : tree unit → tree unit := λ s, (encode $ (decode α s).map n).right,
+  obtain ⟨pf', pn'⟩ : tree.polytime f' ∧ tree.polytime n' := by { split; dsimp [f', n'], complexity, },
+  have H₁ : ∀ x y, decode α x = some y → (f' x = encode (f y) ∧ n' x = n y),
+  { intros x y h, dsimp [f', n'], simp [h, encode], },
+  have H₂ : ∀ x, decode α x = none → f' x = tree.nil ∧ n' x = tree.nil,
+  { intros x h, dsimp [f', n'], simp [h, encode], },
+  have H₃ : ∀ y, f' (encode y) = encode (f y) ∧ n' (encode y) = n y := λ y, H₁ (encode y) _ (tencodable.encodek _),
+  have H₃i : ∀ y m, f'^[m] (encode y) = encode (f^[m] y),
+  { intros y m, induction m with m ih, { simp, },  simp [function.iterate_succ', ih, (H₃ _).1], },
+  have H₄ : ∀ x y m, decode α x = some y → (f'^[m + 1] x = encode (f^[m + 1] y)),
+  { intros x y m h, simp [H₁ x y h, H₃i], },
+  refine ⟨_, tree.polytime.prec pn' pf' _, _⟩, swap,
+  { intro x, simp [(H₃ x).2, has_uncurry.uncurry, H₃i], },
+  cases H with p H, cases polysize.lower α with l hl, cases polysize.decode_upper α with u hu, 
+  use (polynomial.X + (l.comp $ p.comp u)),
+  intros x m hm,
+  cases m, { simp, },
+  cases hd : decode α x with y, { exfalso, simpa [H₂ x hd] using hm, },
+  simp only [H₄ _ _ m hd, (H₁ _ _ hd).2] at ⊢ hm,
+  specialize H _ _ hm,
+  simp only [polynomial.eval_add, polynomial.eval_X, polynomial.eval_comp],
+  apply le_add_left,
+  refine (hl _).trans (l.eval_mono $ H.trans $ p.eval_mono $ hu _ _ hd),
+end
 
-theorem comp₂ 
-  {f : γ₀ → γ₁ → Prop} 
-  {g₀ : α → γ₀} {g₁ : α → γ₁}
-  (hf : polytime_pred f) (hg₀: polytime g₀) (hg₁: polytime g₁) :
-  polytime_pred (λ x, f (g₀ x) (g₁ x)) :=
-  hf.comp $ hg₀.pair $ hg₁
-
-theorem comp₃ 
-  {f : γ₀ → γ₁ → γ₂ → Prop} 
-  {g₀ : α → γ₀} {g₁ : α → γ₁} {g₂ : α → γ₂}
-  (hf : polytime_pred f) (hg₀: polytime g₀) (hg₁: polytime g₁) (hg₂: polytime g₂) :
-  polytime_pred (λ x, f (g₀ x) (g₁ x) (g₂ x)) :=
-  hf.comp $ hg₀.pair $ hg₁.pair $ hg₂
-
-theorem comp₄ 
-  {f : γ₀ → γ₁ → γ₂ → γ₃ → Prop} 
-  {g₀ : α → γ₀} {g₁ : α → γ₁} {g₂ : α → γ₂} {g₃ : α → γ₃}
-  (hf : polytime_pred f) (hg₀: polytime g₀) (hg₁: polytime g₁) (hg₂: polytime g₂) (hg₃: polytime g₃) :
-  polytime_pred (λ x, f (g₀ x) (g₁ x) (g₂ x) (g₃ x)) :=
-  hf.comp $ hg₀.pair $ hg₁.pair $ hg₂.pair $ hg₃
-
-theorem comp₅ 
-  {f : γ₀ → γ₁ → γ₂ → γ₃ → γ₄ → Prop} 
-  {g₀ : α → γ₀} {g₁ : α → γ₁} {g₂ : α → γ₂} {g₃ : α → γ₃} {g₄ : α → γ₄}
-  (hf : polytime_pred f) (hg₀: polytime g₀) (hg₁: polytime g₁) (hg₂: polytime g₂) (hg₃: polytime g₃) (hg₄: polytime g₄) :
-  polytime_pred (λ x, f (g₀ x) (g₁ x) (g₂ x) (g₃ x) (g₄ x)) :=
-  hf.comp $ hg₀.pair $ hg₁.pair $ hg₂.pair $ hg₃.pair $ hg₄
-
-end polytime_pred
+lemma iterate_aux' {α β : Type} [polycodable α] [polycodable β] [polysize α] [polysize β] {n : α → tree unit} {f : α → β → β} {g : α → β} (hn : n ∈ₑ polytime)
+  (hf : f ∈ₑ polytime) (hg : g ∈ₑ polytime) 
+  (hp : ∃ p : mv_polynomial (fin 2) ℕ, ∀ x y (m ≤ (decode ℕ (n x)).iget), size ((f x)^[m] y) ≤ mv_polynomial.eval ![size x, size y] p) :
+  polytime.mem (λ x, (f x)^[(decode ℕ (n x)).iget] (g x)) :=
+begin
+  set f' := λ xy : α × β, (xy.1, f xy.1 xy.2),
+  have pf' : f' ∈ₑ P := by { dsimp [f'], complexity, },
+  have hf' : ∀ n x y, f'^[n] (x, y) = (x, (f x)^[n] y),
+  { intros n x y, induction n with n ih generalizing y, { simp, }, { simp [ih], } }, 
+  have := iterate_aux (λ xy, n (prod.fst xy)) f' (by complexity) pf' _,
+  { convert (complexity_class.mem.snd.comp this).comp (polytime.id'.pair hg),
+    ext x, generalize : g x = y, dsimp only [id, decode], simp [hf'], },
+  cases hp with p hp,
+  use (mv_polynomial.X 0 + p).to_polynomial,
+  rintros ⟨x₁, x₂⟩ m hm,
+  simp at hm ⊢,
+  refine trans _ (mv_polynomial.le_to_polynomial_of_le_sum₂ _ _ _),
+  simpa [hf'] using hp x₁ x₂ m hm,
+end
